[ refactor ] archive some and rename folders

implementation/compiler/stlc.rkt
@@ -1,0 +1,21 @@
+#lang racket
+
+(require
+  (for-syntax syntax/parse)
+  (for-meta 2 racket/base syntax/parse))
+
+(provide (except-out (all-from-out racket) #%app))
+
+(provide (rename-out [app/tc #%app]))
+
+(provide M)
+
+(define-syntax (M stx)
+  (syntax-parse stx
+    ([_ e1 e2] (syntax/loc stx (list e1 e2)))))
+
+(define-syntax (app/tc stx)
+  (syntax-parse stx #:literals (M)
+    ([_ (M e1 e2) e] (syntax/loc stx (cons (#%app e1 e) (#%app e2 e))))
+    ([_ e1 e2 ...] (syntax/loc stx (#%app e1 e2 ...)))
+    ))
