implementation/compiler/test.rkt
@@ -1,0 +1,5 @@
+#lang s-exp "stlc.rkt"
+
+((M (λ (x) x)
+    (λ (x) (+ x 1)))
+ 2)
