archive2/core+bidir+record+unified/Proof/Typing.v
@@ -5,8 +5,11 @@ Require Import Language.
 Require Import Tactical.
 Require Import Subtyping.Subtyping.
 Require Import Appsub.
+Require Import Subtyping.Unisub.
+Require Import Disjoint.
 Require Import Value.
 Require Import PrincipalTyping.
+Require Import Consistent.
 
 
 Import ListNotations.
@@ -28,6 +31,9 @@ Inductive typing : ctx -> term -> mode -> type -> Prop :=
     (forall x, x \notin L ->
           typing ((one (x, A)) ++ T) (open e (Fvar x)) Chk B) ->
     typing T (Lam A e B) Inf (Arr A B)
+| Ty_Rcd : forall T e l A,
+    typing T e Inf A ->
+    typing T (Fld l e) Inf (Rcd l A)
 | Ty_Ann : forall T A e,
     typing T e Chk A ->
     typing T (Ann e A) Inf A
@@ -36,10 +42,22 @@ Inductive typing : ctx -> term -> mode -> type -> Prop :=
     typing T e2 Inf B ->
     uunisub A (uP (Avt B)) (Some C) ->
     typing T (App e1 e2) Inf C
+| Ty_Prj : forall T e l A B,
+    typing T e Inf A ->
+    uunisub A (uP (Alt l)) (Some B) ->
+    typing T (Prj e l) Inf B
 | Ty_Mrg : forall T A B e1 e2,
+    disjoint A B ->
     typing T e1 Inf A ->
     typing T e2 Inf B ->
     typing T (Mrg e1 e2) Inf (And A B)
+| Ty_Mrg_Uv : forall T A B u1 u2,
+    uniq T ->
+    uvalue u1 -> uvalue u2 ->
+    consistent u1 u2 ->
+    typing nil u1 Inf A ->
+    typing nil u2 Inf B ->
+    typing T (Mrg u1 u2) Inf (And A B)
 | Ty_Sub : forall T e A B,
     typing T e Inf A ->
     sub A B ->
@@ -54,17 +72,46 @@ Notation "T ⊢ e ⇐ A" := (typing T e Chk A) (at level 50).
 
 Lemma typing_to_ptype :
   forall u A,
-    value u ->
+    uvalue u ->
     typing nil u Inf A ->
     ptype u A.
 Proof.
-  introv Val Typ. gen A.
-  induction Val; intros.
-  - dependent destruction Typ; eauto.
-  - dependent destruction Typ; eauto.
+  introv Uval Typ. gen A.
+  induction Uval; intros;
+    dependent destruction Typ; eauto.
 Qed.
 
 Hint Resolve typing_to_ptype : core.
+
+(** * Typing & Consistent *)
+
+(** ** Reflexivity *)
+
+(** Well-typed values are consistent with themselves *)
+
+Lemma consistent_reflexivity :
+  forall v A,
+    typing nil v Inf A ->
+    value v ->
+    consistent v v.
+Proof.
+  introv Typ Val. gen A.
+  induction Val; eauto; intros.
+  dependent destruction Typ; eauto.
+  Case "Merge".  
+  dependent destruction Typ.
+  - SCase "Disjoint".
+    assert (consistent v1 v2) by (eapply Con_Dj; eauto).
+    eapply Con_Mrg_L; eauto.
+    eapply Con_Mrg_R; eauto.
+    now apply consistent_symmetry.
+  - SCase "Consistent".
+    eapply Con_Mrg_L; eauto.
+    eapply Con_Mrg_R; eauto.
+    now apply consistent_symmetry.
+Qed.
+
+Hint Resolve consistent_reflexivity : core.
 
 (** * Typing & LC *)
 
