archive2/core+bidir+record+unified/Proof/Language.v
@@ -1,0 +1,187 @@
+(** This file is syntax of Applicative Intersection Types, which is a extension of "Disjoint Intersection Types"
+
+What makes this calculus different from classical simply typed lambda calculus
+
+- It has intersection types
+- It has merge operator (create inhabitants of intersection types)
+- It has subtyping (BCD-style: allow distribuivity upon function types and intersection types)
+- It's type safe: we will prove determinism, preservation and progress
+- Enhanced subtyping algorithms can solve overloading problems
+
+ *)
+
+Require Import Metalib.Metatheory.
+Require Import Coq.Program.Equality.
+Require Import Coq.Strings.String.
+Require Import Tactical.
+
+Import ListNotations.
+
+Set Printing Parentheses.
+
+(** * Types
+
+[type] is:
+
+- [Int] is integer type
+- [Top] is top type (supertype of all types)
+- [Arr] is function type
+- [And] is intersection type
+
+*)
+
+Definition label := nat.
+
+Inductive type : Set :=
+| Int : type
+| Top : type          
+| Arr : type -> type -> type
+| And : type -> type -> type
+| Rcd : label -> type -> type.
+
+Hint Constructors type : core.
+
+(** Notation is only used for prettifying goals, we never explicity write customized notation *)
+
+Notation "A → B" := (Arr A B) (at level 20).
+Notation "A & B" := (And A B) (at level 20).
+Notation "{ l : A }" := (Rcd l A) (at level 20).
+
+(** * Terms
+
+[term] is :
+
+- [Lit] for integers: 1, 2, 3 ...
+- [Bvar] and [Fvar] for binded variables and free variables in locally nameless representation
+- [Lam] for lambda: \x: A. e : B
+- [App] for application: e1 e2
+- [Mrg] for merge operator, which creates inhabitants of intersection types: e1 ,, e2
+- [Ann] for annotated terms: e : A
+
+*)
+
+Inductive term : Set :=
+| Lit : nat -> term
+| Bvar : nat -> term
+| Fvar : var -> term
+| Lam : type -> term -> type -> term
+| App : term -> term -> term
+| Mrg : term -> term -> term
+| Ann : term -> type -> term
+| Fld : label -> term -> term
+| Prj : term -> label -> term.
+
+Hint Constructors term : core.
+
+Notation "e ∷ A" := (Ann e A) (at level 20).
+Notation "ƛ A . e : B" := (Lam A e B) (at level 20).
+Notation "{ l = e }" := (Fld l e) (at level 20).
+Notation "e ◍ l" := (Prj e l) (at level 20).
+
+(** coerce atom x to (Fvar x) *)
+
+Check (Prj (Fld 1 (Lit 1)) 1).
+
+Coercion Fvar : atom >-> term.
+
+(** * Size of types and terms *)
+
+(** [size_type] and [size_term] are defined for more powerful induction principle: induction on size *)
+
+Fixpoint size_type (A : type) {struct A} : nat :=
+  match A with
+  | Int => 1
+  | Top => 1
+  | Arr A B => 1 + (size_type A) + (size_type B)
+  | And A B => 1 + (size_type A) + (size_type B)
+  | Rcd l A => 1 + (size_type A)
+  end.
+
+Fixpoint size_term (e : term) {struct e} : nat :=
+  match e with
+  | Lit n => 1
+  | Bvar n => 1
+  | Fvar x => 1
+  | Lam A e B => 1 + (size_type A) + (size_term e) + (size_type B)
+  | App e1 e2 => 1 + (size_term e1) + (size_term e2)
+  | Mrg e1 e2 => 1 + (size_term e1) + (size_term e2)
+  | Ann e A => 1 + (size_term e) + (size_type A)
+  | Fld l e => 1 + (size_term e)
+  | Prj e l => 1 + (size_term e)
+  end.
+
+(** induction on size *)
+
+Ltac ind_type_size s :=
+  assert (SizeInd: exists i, s < i) by eauto;
+  destruct SizeInd as [i SizeInd];
+  repeat match goal with
+         | [ h : type |- _ ] => (gen h)
+         end;
+  induction i as [|i IH]; [
+      intros; match goal with
+              | [ H : _ < 0 |- _ ] => (dependent destruction H)
+              end
+    | intros ].
+
+(** * Substituion *)
+
+Fixpoint substitution (z : atom) (u : term) (e : term) {struct e} : term :=
+  match e with
+  | Lit n => Lit n
+  | Bvar i => Bvar i
+  | Fvar x => if x == z then u else (Fvar x)
+  | Lam A e B => Lam A (substitution z u e) B
+  | App e1 e2 => App (substitution z u e1) (substitution z u e2)
+  | Mrg e1 e2 => Mrg (substitution z u e1) (substitution z u e2)
+  | Ann e A => Ann (substitution z u e) A
+  | Fld l e => Fld l (substitution z u e)
+  | Prj e l => Prj (substitution z u e) l
+  end.
+
+Notation "{ z ↦ u } e" := (substitution z u e) (at level 69).
+
+(** * Free variables *)
+
+Fixpoint fv (e : term) {struct e} : atoms :=
+  match e with
+  | Lit n => empty
+  | Bvar i => empty
+  | Fvar x => singleton x
+  | Lam A e B => fv e
+  | App e1 e2 => (fv e1) `union` (fv e2)
+  | Mrg e1 e2 => (fv e1) `union` (fv e2)
+  | Ann e A => fv e
+  | Fld l e => fv e
+  | Prj e l => fv e
+  end.
+
+(** * Context *)
+
+Definition ctx : Set := list (var * type).
+
+(** * Opening *)
+
+Fixpoint open_rec (k : nat) (u : term) (e : term) {struct e} : term :=
+  match e with
+  | Lit n => Lit n
+  | Bvar i => if k == i then u else (Bvar i)
+  | Fvar x => Fvar x
+  | Lam A e B => Lam A (open_rec (S k) u e) B
+  | App e1 e2 => App (open_rec k u e1) (open_rec k u e2)
+  | Mrg e1 e2 => Mrg (open_rec k u e1) (open_rec k u e2)
+  | Ann e A => Ann (open_rec k u e) A
+  | Fld l e => Fld l (open_rec k u e)
+  | Prj e l => Prj (open_rec k u e) l
+  end.
+
+Definition open e u := open_rec 0 u e.
+
+(** Auxiliary functions for building contexts automatically *)
+
+Ltac gather_atoms ::=
+  let A := gather_atoms_with (fun x : atoms => x) in
+  let B := gather_atoms_with (fun x : atom => singleton x) in
+  let C := gather_atoms_with (fun x : list (atom * type) => dom x) in
+  let D := gather_atoms_with (fun x : term => fv x) in
+  constr:(A `union` B `union` C `union` D).
