archive2/core/Proof/Reduction.v
@@ -1,0 +1,408 @@
+Require Import Metalib.Metatheory.
+Require Import Metalib.LibTactics.
+Require Import Coq.Program.Equality.
+Require Import Coq.Program.Tactics.
+Require Import Strings.String.
+Require Import Psatz.
+
+Require Import Language.
+Require Import Tactical.
+Require Import Subtyping.Subtyping.
+Require Import Subtyping.Splitable.
+Require Import Subtyping.Toplike.
+Require Import Appsub.
+
+Require Import Value.
+Require Import Disjoint.
+Require Import PrincipalTyping.
+Require Import Consistent.
+Require Import Typing.
+Require Import Casting.
+Require Import LocallyNameless.
+Require Import Application.
+
+(** * Definition *)
+
+Inductive step : term -> term -> Prop :=
+| St_Lit : forall n,
+    step (Lit n) (Ann (Lit n) Int)
+| St_Lam : forall e A B,
+    step (Lam A e B) (Ann (Lam A e B) (Arr A B))
+| St_Spl : forall p A A1 A2,
+    pvalue p ->
+    splitable A A1 A2 ->
+    step (Ann p A) (Mrg (Ann p A1) (Ann p A2))
+| St_App : forall v vl e,
+    value v -> value vl ->
+    papp v vl e ->
+    step (App v vl) e
+| St_Val : forall v v' A,
+    value v ->
+    casting v A v' ->
+    step (Ann v A) v'
+| St_Ann : forall e e' A,
+    not (pvalue e) ->
+    step e e' ->
+    step (Ann e A) (Ann e' A)
+| St_App_L : forall e1 e1' e2,
+    lc e2 ->
+    step e1 e1' ->
+    step (App e1 e2) (App e1' e2)
+| St_App_R : forall v e2 e2',
+    value v ->
+    step e2 e2' ->
+    step (App v e2) (App v e2')
+| St_Mrg : forall e1 e1' e2 e2',
+    step e1 e1' ->
+    step e2 e2' ->
+    step (Mrg e1 e2) (Mrg e1' e2')         
+| St_Mrg_L : forall e1 v e1',
+    value v ->
+    step e1 e1' ->
+    step (Mrg e1 v) (Mrg e1' v)
+| St_Mrg_R : forall v e2 e2',
+    value v ->
+    step e2 e2' ->
+    step (Mrg v e2) (Mrg v e2').
+
+Hint Constructors step : core.
+
+Notation "e ⟾ e'" := (step e e') (at level 68).
+
+(** * Value *)
+
+Lemma value_no_step :
+  forall v,
+    value v -> forall e, ~ step v e.
+Proof.
+  introv Val.
+  induction v; intros; eauto.
+  - intros St.
+    dependent destruction Val. dependent destruction St; eauto.
+    + eapply IHv1; eauto.
+    + eapply IHv1; eauto.
+    + eapply IHv2; eauto.
+  - dependent destruction Val.
+    destruct H.
+    + intros St. dependent destruction St; eauto.
+    + intros St. dependent destruction St; eauto.
+Qed.
+
+Lemma step_lc :
+  forall e e',
+    lc e -> step e e' -> lc e'.
+Proof.
+  introv Lc St. gen e'.
+  induction Lc; intros;
+    try solve [dependent destruction St; eauto 3].
+  - dependent destruction St. eapply Lc_Ann. eapply Lc_Lam; eauto.
+  - dependent destruction St; try solve [econstructor; eauto].
+    pose proof (papp_lc e1 e2 e). eauto 3.
+  - dependent destruction St; econstructor; eauto.
+  - dependent destruction St.
+    + econstructor; eapply Lc_Ann; eapply lc_pvalue; eauto.
+    + eapply casting_lc; eauto.
+    + econstructor. eauto.
+Qed. 
+
+Lemma step_uvalue :
+  forall u u',
+    uvalue u -> step u u' -> uvalue u'.
+Proof.
+  introv Uv St. gen u'.
+  induction Uv; intros.
+  - dependent destruction St; eauto.
+    eapply Uv_Ann. eapply step_lc; eauto.
+  - dependent destruction St; eauto.
+Qed.
+
+Hint Resolve step_uvalue : core.
+
+(** * Determinism *)
+
+Section determinism.
+
+Ltac solver1 := try solve [match goal with
+                           | [Val: value ?v, St: step ?v _ |- _] =>
+                               (pose proof (value_no_step _ Val _ St); contradiction)
+                           end].
+
+Theorem determinism:
+  forall e e1 e2 A,
+    typing nil e A ->
+    step e e1 -> step e e2 -> e1 = e2.
+Proof.
+  introv Typ St1 St2. gen e2 A.
+  dependent induction St1; intros.
+  - dependent destruction St2; eauto.
+  - dependent destruction St2; eauto.
+  - dependent destruction St2; eauto.
+    subst_splitable. reflexivity.
+  - dependent destruction St2; solver1.
+    pose proof (papp_determinism v vl e). eauto.
+  - dependent destruction St2; eauto; solver1.
+    dependent destruction Typ.
+    eapply casting_determinism; eauto.
+  - dependent destruction St2; eauto; solver1.
+    f_equal. dependent destruction Typ; eauto.
+  - dependent destruction St2; solver1.
+    f_equal. dependent destruction Typ; eauto.
+  - dependent destruction St2; solver1.
+    f_equal. dependent destruction Typ; eauto.
+  - dependent destruction St2; solver1.
+    dependent destruction Typ;
+      f_equal; eauto.
+  - dependent destruction St2; solver1.
+    dependent destruction Typ;
+      f_equal; eauto.
+  - dependent destruction St2; solver1.
+    dependent destruction Typ;
+      f_equal; eauto.
+Qed.
+
+End determinism.
+
+(** * Consistent *)
+
+Inductive step_or_value : term -> term -> Prop :=
+| Sv_V : forall v, value v -> step_or_value v v
+| Sv_S : forall e1 e2, step e1 e2 -> step_or_value e1 e2.
+
+Hint Constructors step_or_value : core.
+
+Lemma size_term_lg_z :
+  forall e, size_term e > 0.
+Proof.
+  introv.
+  dependent induction e; try solve [eauto | simpl; lia].
+Qed.
+
+Hint Resolve size_term_lg_z : core.
+
+Lemma size_term_lg_z_any1 :
+  forall e1 e2,
+    size_term e1 < (size_term e2 + size_term e1).
+Proof.
+  introv.
+  assert (size_term e2 > 0). eapply size_term_lg_z.
+  lia.
+Qed.
+
+Lemma size_term_lg_z_any2 :
+  forall e1 e2,
+    size_term e1 < (size_term e1 + size_term e2).
+Proof.
+  introv.
+  assert (size_term e2 > 0). eapply size_term_lg_z.
+  lia.
+Qed.
+
+Hint Resolve size_term_lg_z_any1 : core.
+Hint Resolve size_term_lg_z_any2 : core.
+
+Section step_consistent.
+
+Ltac solver1 := match goal with
+                | [St: step (Ann (Lam _ _ _) _) _ |- _] => (dependent destruction St; eauto)
+                end.
+
+Ltac solver2 := match goal with
+                | [St: step (Ann _ _) _ |- _] => (dependent destruction St; eauto)
+                end.
+
+Ltac solver3 := match goal with
+                | [Val: value ?v, St: step ?v _ |- _] =>
+                    (pose proof (value_no_step _ Val _ St); contradiction)
+                end.
+
+Ltac solver4 IHC IH :=
+  eapply IHC; eauto; intros; match goal with
+                             | St: step ?e ?e' |- _ => eapply (IH e e'); eauto; simpl; lia
+                             end.
+
+Lemma step_consistent :
+  forall e1 e2 e1' e2' A B,
+    uvalue e1 -> uvalue e2 ->
+    typing nil e1 A -> typing nil e2 B ->
+    consistent e1 e2 ->
+    step_or_value e1 e1' -> step_or_value e2 e2' ->
+    (forall e e' A, size_term e < (size_term e1 + size_term e2) ->
+        typing nil e A -> step e e' -> (exists C, typing nil e' C /\ isosub C A)) ->
+    consistent e1' e2'.
+Proof.
+  introv Uv1 Uv2 Typ1 Typ2 Con Sv1 Sv2 IH. gen A B e1' e2'.
+  dependent induction Con; intros; eauto.
+  - Case "Lam Lam".
+    dependent destruction Sv1; dependent destruction Sv2; eauto; try solve [solver1].
+    dependent destruction Typ1. dependent destruction Typ2.
+    solver1. solver1. eapply Con_Mrg_L; eauto.
+  - Case "Anno Anno".
+    dependent destruction Sv1; dependent destruction Sv2; eauto; try solve [solver2].
+    dependent destruction Typ1. dependent destruction Typ2.
+    solver2.
+    * solver2. eapply Con_Mrg_L; eauto.
+    * solver2; try solve [solver3].
+      pose proof (casting_preservation e v' A C) as Cp1.
+      pose proof (casting_preservation e v'0 B C0) as Cp2.
+      destruct Cp1; destruct Cp2; eauto. destruct_conjs.
+      eapply casting_consistent; eauto.      
+    * solver2; try solve [solver3].
+      assert (e' = e'0). eapply determinism; eauto. subst. econstructor; eauto.
+      eapply step_lc; eauto.
+  - Case "Disjoint".    
+    dependent destruction Sv1; dependent destruction Sv2; eauto.
+    + pose proof (step_uvalue _ _ Uv2 H3).
+      eapply IH in H3; eauto; try lia.
+      destruct H3 as [x Typ]; destruct Typ as [Typ Isub].
+      eapply typing_to_ptype in Typ; eauto.
+      eapply typing_to_ptype in Typ2; eauto. subst_ptype.
+      eapply Con_Dj; eauto. eapply disjoint_iso_l; eauto.
+    + pose proof (step_uvalue _ _ Uv1 H2).
+      eapply IH in H2; eauto; try lia.
+      destruct H2 as [x Typ]; destruct Typ as [Typ Isub].
+      eapply typing_to_ptype in Typ; eauto.
+      eapply typing_to_ptype in Typ1; eauto. subst_ptype.
+      eapply Con_Dj; eauto. eapply disjoint_iso_l; eauto.
+    + pose proof (step_uvalue _ _ Uv1 H2).
+      pose proof (step_uvalue _ _ Uv2 H3).
+      eapply IH in H2; eauto; try lia.
+      eapply IH in H3; eauto; try lia.
+      destruct_conjs.
+      eapply typing_to_ptype in Typ1; eauto.
+      eapply typing_to_ptype in Typ2; eauto. repeat subst_ptype.
+      eapply Con_Dj; eauto. eapply disjoint_iso_l; eauto.
+  - Case "Merge L".
+    dependent destruction Sv1; eauto 3.
+    + dependent destruction Typ1;
+        eapply Con_Mrg_L; try solve [solver4 IHCon1 IH | solver4 IHCon2 IH].
+    + dependent destruction Typ1;
+        match goal with
+        | St: step (Mrg _ _) _ |- _ => dependent destruction St
+        end; eapply Con_Mrg_L; try solve [solver4 IHCon1 IH | solver4 IHCon2 IH].
+  - Case "Merge R".
+    dependent destruction Sv2; eauto 3.
+    + dependent destruction Typ2;
+        eapply Con_Mrg_R; try solve [solver4 IHCon1 IH | solver4 IHCon2 IH].
+    + dependent destruction Typ2;
+        match goal with
+        | St: step (Mrg _ _) _ |- _ => dependent destruction St
+        end; eapply Con_Mrg_R; try solve [solver4 IHCon1 IH | solver4 IHCon2 IH].
+Qed.
+    
+End step_consistent.
+
+(** * Preservation *)
+
+Ltac ind_term_size s :=
+  assert (SizeInd: exists i, s < i) by eauto;
+  destruct SizeInd as [i SizeInd];
+  repeat match goal with | [ h : term |- _ ] => (gen h) end;
+  induction i as [|i IH]; [
+      intros; match goal with | [ H : _ < 0 |- _ ] => (dependent destruction H) end
+    | intros ].
+
+Theorem preservation :
+  forall e e' A,
+    typing nil e A ->
+    step e e' ->
+    (exists B, typing nil e' B /\ isosub B A).
+Proof.
+  introv Typ St. gen e' A.
+  ind_term_size (size_term e).
+  dependent destruction Typ; simpl in SizeInd.
+  - Case "Lit".
+    dependent destruction St; eauto.
+  - Case "Var".
+    dependent destruction St.
+  - Case "Lam".
+    dependent destruction St; eauto.
+  - Case "Ann".
+    dependent destruction St.
+    + SCase "Split".
+      exists (And A1 A2). split; eauto.
+      pose proof (sub_inv_splitable_r C A A1 A2) as Sub. destruct Sub; eauto.
+      eapply Ty_Mrg_Uv; eauto.
+    + SCase "Value".
+      eapply casting_preservation; eauto.
+    + SCase "Ann".
+      eapply IH in St; eauto; try lia.
+      destruct St as [B Typ']. destruct Typ' as [Typ'1 Typ'2].
+      pose proof (isosub_to_sub1 _ _ Typ'2).
+      exists A. split; eauto. eapply Ty_Ann; eauto; try solve [eapply sub_transitivity; eauto].
+  - Case "App".
+    dependent destruction St.
+    + pose proof (papp_preservation e1 e2 e) as P.
+      eapply P; eauto.
+    + eapply IH in St; eauto; try lia. destruct_conjs.
+      eapply appsub_iso in H0; eauto. destruct_conjs.
+      eexists; eauto.
+    + eapply IH in St; eauto; try lia. destruct_conjs.
+      eapply appsub_iso in H0; eauto. destruct_conjs.
+      eexists; eauto.
+  - Case "Merge".
+    dependent destruction St.
+    + eapply IH in St1; eauto; try lia.
+      eapply IH in St2; eauto; try lia. destruct_conjs.      
+      eapply disjoint_iso_l in H; eauto.
+    + eapply IH in St; eauto; try lia. destruct_conjs.
+      eapply disjoint_iso_l in H0; eauto.
+    + eapply IH in St; eauto; try lia. destruct_conjs.
+      eapply disjoint_iso_l in H0; eauto.
+  - Case "Merge U".
+    dependent destruction St.    
+    + (* TODO: Automation *)
+      assert (exists C, (typing nil e1' C) /\ (isosub C A)) by (eapply IH; eauto; lia).
+      assert (exists C, (typing nil e2' C) /\ (isosub C B)) by (eapply IH; eauto; lia).
+      destruct_conjs. exists (And H3 H4).
+      pose proof (step_uvalue _ _ H0 St1).
+      pose proof (step_uvalue _ _ H1 St2).
+      split; eauto. eapply Ty_Mrg_Uv; eauto.
+      pose proof (Sv_S _ _ St1) as Sov1.
+      pose proof (Sv_S _ _ St2) as Sov2.
+      pose proof (step_consistent u1 u2 e1' e2' A B H0 H1 Typ1 Typ2 H2 Sov1 Sov2) as Sc.
+      eapply Sc. intros. eapply IH; eauto. lia.
+    + assert (exists C, (typing nil e1' C) /\ (isosub C A)) by (eapply IH; eauto; lia).
+      destruct_conjs. exists (And H4 B).
+      pose proof (step_uvalue _ _ H1 St).
+      split; eauto. eapply Ty_Mrg_Uv; eauto.
+      pose proof (Sv_S _ _ St) as Sov1.
+      pose proof (Sv_V _ H) as Sov2.
+      pose proof (step_consistent u1 u2 e1' u2 A B H1 H2 Typ1 Typ2 H3 Sov1 Sov2) as Sc.
+      eapply Sc; eauto. intros. eapply IH; eauto. lia.
+    + assert (exists C, (typing nil e2' C) /\ (isosub C B)) by (eapply IH; eauto; lia).
+      destruct_conjs. exists (And A H4).
+      pose proof (step_uvalue _ _ H2 St).
+      split; eauto. eapply Ty_Mrg_Uv; eauto.
+      pose proof (Sv_V _ H) as Sov1.
+      pose proof (Sv_S _ _ St) as Sov2.
+      pose proof (step_consistent u1 u2 u1 e2' A B H1 H2 Typ1 Typ2 H3 Sov1 Sov2) as Sc.
+      eapply Sc; eauto. intros. eapply IH; eauto. lia.
+      Unshelve. eauto.
+Qed.
+
+(** * Progress *)
+
+Theorem progress :
+  forall e A,
+    typing nil e A ->
+    value e \/ exists e', step e e'.
+Proof.
+  introv Typ.
+  dependent induction Typ; eauto 3.
+  - Case "Anno".
+    destruct IHTyp as [Val | St] ; eauto.
+    + right. eapply casting_progress in Typ; eauto. destruct Typ.
+      exists x. eapply St_Val; eauto.
+    + destruct (pvalue_decidable e) as [Pv | nPv];
+        destruct (splitable_or_ordinary A) as [Spl | Ord]; eauto.
+      * destruct Pv; right; destruct_conjs; eexists; eauto.
+      * destruct St. right. eexists; eauto.
+      * destruct St. right. eexists; eauto.
+  - Case "App".
+    right. destruct IHTyp1; destruct IHTyp2; eauto 3; try solve [destruct_conjs; eauto].
+    pose proof (papp_progress e1 e2 A B C) as P. destruct P; eauto.
+  - Case "Merge".
+    destruct IHTyp1; destruct IHTyp2; eauto 3; try solve [destruct_conjs; eauto].
+  - Case "Merge V".
+    destruct IHTyp1; destruct IHTyp2; eauto 3; try solve [destruct_conjs; eauto].
+Qed.
