archive2/core/Proof/Typing.v
@@ -1,0 +1,111 @@
+Require Import Metalib.Metatheory.
+Require Import Program.Equality.
+Require Import Strings.String.
+Require Import Language.
+Require Import Tactical.
+Require Import Subtyping.Subtyping.
+Require Import Appsub.
+Require Import Disjoint.
+Require Import Value.
+Require Import PrincipalTyping.
+Require Import Consistent.
+
+
+Import ListNotations.
+
+(** * Definition *)
+
+Inductive typing : ctx -> term -> type -> Prop :=
+| Ty_Int : forall T n,
+    uniq T ->
+    typing T (Lit n) Int
+| Ty_Var : forall T x A,
+    uniq T -> binds x A T ->
+    typing T (Fvar x) A
+| Ty_Lam : forall L T A B C e,
+    (forall x, x \notin L ->
+          typing ((one (x, A)) ++ T) (open e (Fvar x)) C) ->
+    sub C B ->
+    typing T (Lam A e B) (Arr A B)
+| Ty_Ann : forall T A C e,
+    typing T e C ->
+    sub C A ->
+    typing T (Ann e A) A
+| Ty_App : forall T A B C e1 e2,
+    typing T e1 A ->
+    typing T e2 B ->
+    appsub (Some B) A C ->
+    typing T (App e1 e2) C
+| Ty_Mrg : forall T A B e1 e2,
+    disjoint A B ->
+    typing T e1 A ->
+    typing T e2 B ->
+    typing T (Mrg e1 e2) (And A B)
+| Ty_Mrg_Uv : forall T A B u1 u2,
+    uniq T ->
+    uvalue u1 -> uvalue u2 ->
+    consistent u1 u2 ->
+    typing nil u1 A ->
+    typing nil u2 B ->
+    typing T (Mrg u1 u2) (And A B).
+
+Hint Constructors typing : core.
+
+Notation "T ⊢ e ⦂ A" := (typing T e A) (at level 50).
+
+(** * Typing & PrincipalTyping *)
+
+Lemma typing_to_ptype :
+  forall u A,
+    uvalue u ->
+    typing nil u A ->
+    ptype u A.
+Proof.
+  introv Uval Typ. gen A.
+  induction Uval; intros.
+  - dependent destruction Typ; eauto.
+  - dependent destruction Typ; eauto.
+Qed.
+
+Hint Resolve typing_to_ptype : core.
+
+(** * Typing & Consistent *)
+
+(** ** Reflexivity *)
+
+(** Well-typed values are consistent with themselves *)
+
+Lemma consistent_reflexivity :
+  forall v A,
+    typing nil v A ->
+    value v ->
+    consistent v v.
+Proof.
+  introv Typ Val. gen A.
+  induction Val; eauto; intros.
+  Case "Merge".  
+  dependent destruction Typ.
+  - SCase "Disjoint".
+    assert (consistent v1 v2) by (eapply Con_Dj; eauto).
+    eapply Con_Mrg_L; eauto.
+    eapply Con_Mrg_R; eauto.
+    now apply consistent_symmetry.
+  - SCase "Consistent".
+    eapply Con_Mrg_L; eauto.
+    eapply Con_Mrg_R; eauto.
+    now apply consistent_symmetry.
+Qed.
+
+Hint Resolve consistent_reflexivity : core.
+
+(** * Typing & LC *)
+
+Lemma typing_to_lc :
+  forall T e A,
+    typing T e A -> lc e.
+Proof.
+  introv Typ.
+  induction Typ; try solve [econstructor; eauto].
+Qed.
+
+Hint Resolve typing_to_lc : core.
