core+record+disjoint/Proof/Application.v
@@ -1,0 +1,826 @@
+Require Import Metalib.Metatheory.
+Require Import Metalib.LibTactics.
+Require Import Coq.Program.Equality.
+Require Import Coq.Program.Tactics.
+Require Import Strings.String.
+Require Import Lia.
+
+Require Import Language.
+Require Import Tactical.
+Require Import Subtyping.Subtyping.
+Require Import Subtyping.Splitable.
+Require Import Subtyping.Toplike.
+Require Import Subtyping.Unisub.
+Require Import Appsub.
+
+Require Import Value.
+Require Import Disjoint.
+Require Import PrincipalTyping.
+Require Import Consistent.
+Require Import Typing.
+Require Import Casting.
+Require Import LocallyNameless.
+
+(** * Definition *)
+
+(** instead of using principal typing to get the type, we can define a function 
+    atype : vl -> arg
+    atype v = Some A
+    atype l = Some l
+ *)
+
+(** value and label *)
+
+Inductive vl : Set :=
+| Av : term -> vl
+| Al : label -> vl.
+
+Hint Constructors vl : core.
+
+(** I'm confused a little bit and try to think why not let merge to be general one (work both on type and label),
+    Since we can't allow label to be merged, so merge case only account for types 
+*)
+
+Inductive atype : vl -> arg -> Prop :=
+| At_Ann : forall e A,
+    atype (Av (Ann e A)) (Avt A)
+| At_Rcd : forall e l A,
+    atype (Av e) (Avt A) ->
+    atype (Av (Fld l e)) (Avt (Rcd l A))
+| At_Mrg : forall e1 e2 A1 A2,
+    atype (Av e1) (Avt A1) ->
+    atype (Av e2) (Avt A2) ->
+    atype (Av (Mrg e1 e2)) (Avt (And A1 A2))
+| At_Lbl : forall l,
+    atype (Al l) (Alt l).
+
+Hint Constructors atype : core.
+
+(* Fixpoint selector (t : type) : bool := *)
+(*   match t with *)
+(*   | Arr _ _ => true *)
+(*   | Rcd _ _ => true *)
+(*   | _       => false *)
+(*   end. *)
+
+Inductive selectorT : type -> type -> Prop :=
+| SeT_Arr : forall A B,
+    selectorT (Arr A B) B
+| SeT_Rcd : forall l A,
+    selectorT (Rcd l A) A.
+
+Hint Constructors selectorT : core.
+
+Inductive papp : term -> vl -> term -> Prop :=
+(* | Pa_Lit_Tl : forall A B v n, *)
+(*     toplike B -> *)
+(*     papp (Ann (Lit n) (Arr A B)) (Av v) *)
+(*          (Ann (Lit 1) B) *)
+(* | Pa_Lit_Tl_R : forall A n l, *)
+(*     toplike A -> *)
+(*     papp (Ann (Lit n) (Rcd l A)) (Al l) *)
+(*          (Ann (Lit 1) A) *)
+(* | Pa_Lam_Tl : forall A B C D e v, *)
+(*     lc (Lam A e B) -> *)
+(*     toplike D -> *)
+(*     papp (Ann (Lam A e B) (Arr C D)) (Av v) *)
+(*          (Ann (Lit 1) D) *)
+(* | Pa_Lam_Tl_R : forall A B C l e, *)
+(*     lc (Lam A e B) -> *)
+(*     toplike C -> *)
+(*     papp (Ann (Lam A e B) (Rcd l C)) (Al l) *)
+(*          (Ann (Lit 1) C) *)
+| Pa_Top : forall p A B vl,
+    selectorT A B -> toplike B ->
+    papp (Ann p A) vl (Ann (Lit 1) B)
+| Pa_Lam : forall A B C D v v' e,
+    lc (Lam A e B) ->
+    casting v A v' ->
+    not (toplike D) ->
+    papp (Ann (Lam A e B) (Arr C D)) (Av v)
+         (Ann (open e v') D)
+| Pa_Rcd : forall v l,
+    papp (Fld l v) (Al l) v
+| Pa_Mrg_L : forall v1 v2 A B vl TA e,
+    ptype v1 A -> ptype v2 B ->
+    atype vl TA ->
+    not (uunisub B (uV TA) None) ->
+    papp v1 vl e ->
+    papp (Mrg v1 v2) vl e
+| Pa_Mrg_R : forall v1 v2 A B vl TA e,
+    ptype v1 A -> ptype v2 B ->
+    atype vl TA ->
+    not (uunisub A (uV TA) None) ->
+    papp v2 vl e ->
+    papp (Mrg v1 v2) vl e
+| Pa_Mrg_P : forall v1 v2 A B vl TA e1 e2,
+    ptype v1 A -> ptype v2 B ->
+    atype vl TA ->
+    uunisub A (uV TA) None ->
+    uunisub B (uV TA) None ->
+    papp v1 vl e1 ->
+    papp v2 vl e2 ->
+    papp (Mrg v1 v2) vl (Mrg e1 e2).
+
+Hint Constructors papp : core.
+
+Notation "v · vl ⟹ e" := (papp v vl e) (at level 69).
+
+(** * Determinism *)
+
+Lemma atype_determinism :
+  forall vl TA1 TA2,
+    atype vl TA1 ->
+    atype vl TA2 ->
+    TA1 = TA2.
+Proof.
+  introv At1 At2. gen TA2.
+  dependent induction At1; intros.
+  - dependent destruction At2; eauto.
+  - dependent destruction At2; eauto.
+    pose proof (IHAt1 _ At2) as IH.
+    dependent destruction IH; eauto.
+  - dependent destruction At2.
+    pose proof (IHAt1_1 _ At2_1) as IH1.
+    pose proof (IHAt1_2 _ At2_2) as IH2.
+    dependent destruction IH1. dependent induction IH2.
+    auto.
+  - dependent destruction At2; eauto.
+Qed.
+
+Ltac subst_atype :=
+  match goal with
+  | [H1: atype ?vl ?TA1, H2: atype ?vl ?TA2 |- _] =>
+      (pose proof (atype_determinism _ _ _ H1 H2) as Eqs; subst; clear H2)
+  end.
+
+Lemma typing_to_atype :
+  forall v A,
+    value v ->
+    typing nil v Inf A ->
+    atype (Av v) (Avt A).
+Proof.
+  introv Val Typ. gen A.
+  induction Val; intros.
+  - dependent destruction Typ; eauto.
+  - dependent destruction Typ; eauto.
+  - dependent destruction Typ; eauto.
+Qed.
+
+Hint Resolve typing_to_atype : core.
+
+(** Well-typed application term doesn't ensure that all subterms of function can accept its argument,
+    but ensures part of its functions can accept *)
+
+(** Notation: automation heavily relies on [contra_appsub] *)
+
+Section papp_determinism.
+
+Ltac solver1 := repeat match goal with
+                       | Typ: typing nil ?v Inf ?A, Val: value ?v, Pt: ptype ?v _ |- _ =>
+                           pose proof (typing_to_ptype _ _ (value_is_uvalue _ Val) Typ);
+                           subst_ptype; clear Pt
+                       | Typ: typing nil ?v Inf ?A, Val: value ?v, At: atype (Av ?v) _ |- _ =>
+                           pose proof (typing_to_atype _ _ Val Typ);
+                           subst_atype; clear At
+                       end;
+                match goal with
+                | As: appsub _ _ _ |- _ => (dependent destruction As; eauto)
+                end.
+
+Ltac solver2 := match goal with
+                | SeT : selectorT _ _ |- _ => dependent destruction SeT
+                end.
+
+Lemma papp_determinism_v :
+  forall f v e1 e2 A B C,
+    value f -> value v ->
+    typing nil f Inf A -> typing nil v Inf B ->
+    appsub (Some (Avt B)) A C ->
+    papp f (Av v) e1 ->
+    papp f (Av v) e2 ->
+    e1 = e2.
+Proof.
+  introv Valf Val Typ1 Typ2 As P1 P2. gen e2 A B C.
+  dependent induction P1; intros.
+  - Case "Toplike".
+    dependent destruction Valf. destruct H1;
+      dependent destruction H; dependent destruction P2; try solve [solver2; eauto]; eauto.
+  - Case "Lam".
+    dependent destruction P2; try solve [solver2; eauto]; eauto.
+    repeat (f_equal). eapply casting_determinism; eauto.
+  - Case "Merge L".
+    dependent destruction P2;
+      repeat subst_ptype; subst_atype;
+      dependent destruction Valf; dependent destruction Typ1; solver1.
+  - Case "Merge R".
+    dependent destruction P2; eauto;
+      repeat subst_ptype; subst_atype;
+      dependent destruction Valf; dependent destruction Typ1; solver1.
+  - Case "Merge P".
+    dependent destruction P2; eauto;
+      repeat subst_ptype; subst_atype;
+      dependent destruction Valf; dependent destruction Typ1; solver1.
+    + f_equal; solver1.
+    + f_equal; solver1.
+Qed.
+
+Lemma papp_determinism_l :
+  forall v l e1 e2 A B,
+    value v ->
+    typing nil v Inf A ->
+    appsub (Some (Alt l)) A B ->
+    papp v (Al l) e1 ->
+    papp v (Al l) e2 ->
+    e1 = e2.
+Proof.
+  introv Val Typ As P1 P2. gen e2 A B.
+  dependent induction P1; intros.
+  - Case "Toplike".
+    dependent destruction Val. destruct H1;
+      dependent destruction H; dependent destruction P2; try solve [solver2; eauto]; eauto.
+  - Case "Prj".
+    dependent destruction P2; eauto.
+  - Case "Mrg L".
+    dependent destruction P2;
+      repeat subst_ptype; subst_atype;
+      match goal with
+      | At: atype (Al _) _ |- _ => dependent destruction At
+      end; eauto;
+      dependent destruction Val; dependent destruction Typ; solver1.
+  - Case "Mrg R".
+    dependent destruction P2;
+      repeat subst_ptype; subst_atype;
+      match goal with
+      | At: atype (Al _) _ |- _ => dependent destruction At
+      end; eauto;
+      dependent destruction Val; dependent destruction Typ; solver1.
+  - Case "Mrg P".
+    dependent destruction P2;
+      repeat subst_ptype; subst_atype;
+      match goal with
+      | At: atype (Al _) _ |- _ => dependent destruction At
+      end; eauto;
+      dependent destruction Val; dependent destruction Typ; solver1.
+    + f_equal; eauto.
+    + f_equal; eauto.
+Qed.
+      
+End papp_determinism.
+
+(** * App & Value *)
+
+Lemma papp_lc_v :
+  forall v vl e,
+    lc v -> lc vl ->
+    papp v (Av vl) e ->
+    lc e.
+Proof.
+  introv Lc Lcl Pa.
+  dependent induction Pa; try solve [econstructor; eauto 3].
+  - econstructor. eapply open_abs; eauto 3.
+    eapply casting_lc; eauto.
+  - dependent destruction Lc; eauto 3.
+  - dependent destruction Lc; eauto 3.
+Qed.
+
+Lemma papp_lc_l :
+  forall v vl e,
+    lc v ->
+    papp v (Al vl) e ->
+    lc e.
+Proof.
+  introv Lc Pa.
+  dependent induction Pa; try solve [econstructor; eauto 3].
+  - dependent destruction Lc. assumption.
+  - dependent destruction Lc; eauto 3.
+  - dependent destruction Lc; eauto 3.
+Qed.
+
+(** * App & Consistent *)
+
+(** Automating this lemma is tricky for it has "four" irrelevant cases *)
+
+Section papp_consistent.
+
+Ltac solver1 := try solve [eapply Con_Dj; eauto; eapply disjoint_toplike; eauto 3].
+Ltac solver2 := try solve [eapply Con_Dj; eauto; eapply disjoint_symmetry; eapply disjoint_toplike; eauto 3].
+Ltac solver3 := try solve [match goal with
+                           | [Val: value (Mrg ?v1 ?v2),
+                              Con: consistent _ (Mrg ?v1 ?v2),
+                              Typ: typing nil (Mrg ?v1 ?v2) Inf _ |- _] =>
+      (dependent destruction Val; eapply consistent_inv_merge_r in Con; destruct Con; dependent destruction Typ; eauto 4)
+                              end].
+Ltac solver4 := try solve [match goal with
+                           | [Val: value (Mrg ?v1 ?v2),
+                              Con: consistent (Mrg ?v1 ?v2) _,
+                              Typ: typing nil (Mrg ?v1 ?v2) Inf _ |- _] =>
+      (dependent destruction Val; eapply consistent_inv_merge_l in Con; destruct Con; dependent destruction Typ; eauto 4)
+                            end].
+Ltac solver5 := try solve [match goal with
+                           | Typ: typing nil (Fld ?l ?v) Inf _,
+                              Val: value (Fld ?l ?v) |- _=> pose proof (typing_to_ptype _ _ (value_is_uvalue _ Val) Typ) as TEMPPT;
+                                                          dependent destruction TEMPPT; solver1
+                           end].
+Ltac solver6 := try solve [match goal with
+                           | Typ: typing nil (Fld ?l ?v) Inf _,
+                              Val: value (Fld ?l ?v) |- _=> pose proof (typing_to_ptype _ _ (value_is_uvalue _ Val) Typ) as TEMPPT;
+                                                          dependent destruction TEMPPT; solver2
+                           end].
+                                    
+
+Lemma papp_consistent_v :
+  forall v1 v2 vl e1 e2 A B C,
+    value v1 -> value v2 -> value vl ->
+    typing nil v1 Inf A ->
+    typing nil v2 Inf B ->
+    typing nil vl Inf C ->
+    papp v1 (Av vl) e1 ->
+    papp v2 (Av vl) e2 ->
+    consistent v1 v2 ->
+    consistent e1 e2.
+Proof.
+  introv Val1 Val2 Vall Typ1 Typ2 Typl P1 P2 Con. gen A B C.
+  dependent induction P1.
+  - Case "Toplike".
+    dependent induction P2; intros; solver1; solver3.
+  - Case "Lam".
+    dependent induction P2; intros; solver2; solver3.
+    dependent destruction Con; eauto.
+    + assert (v' = v'0). eapply casting_determinism; eauto. subst. eapply Con_Ann; eauto 4.
+    + assert (v' = v'0). eapply casting_determinism; eauto. subst. eapply Con_Ann; eauto 4.
+    + repeat (dependent destruction Typ1; dependent destruction Typ2).
+      repeat match goal with
+               [H: ptype _ _ |- _] => (dependent destruction H)
+             end.
+      eapply Con_Dj; eauto.
+  - Case "Merge L".
+    dependent induction P2; intros; solver4.
+  - Case "Merge R".
+    dependent induction P2; intros; solver4.
+  - Case "Merge P".
+    dependent induction P2; intros; eapply Con_Mrg_L; solver4.
+Qed.
+
+Lemma papp_consistent_l :
+  forall v1 v2 e1 e2 A B l,
+    value v1 -> value v2 ->
+    typing nil v1 Inf A ->
+    typing nil v2 Inf B ->
+    papp v1 (Al l) e1 ->
+    papp v2 (Al l) e2 ->
+    consistent v1 v2 ->
+    consistent e1 e2.
+Proof.
+  introv Val1 Val2 Typ1 Typ2 P1 P2 Con. gen A B.
+  dependent induction P1.
+  - Case "Toplike".
+    dependent induction P2; intros; solver1; solver3; solver5.
+  - Case "Rcd".
+    dependent induction P2; intros; solver3; solver6.
+    dependent destruction Con; eauto.
+    dependent destruction H. dependent destruction H0.
+    eapply Con_Dj; eauto. dependent destruction H1; eauto.
+    contradiction.
+  - Case "Merge L".
+    dependent induction P2; intros; solver4.
+  - Case "Merge R".
+    dependent induction P2; intros; solver4.
+  - Case "Merge P".
+    dependent induction P2; intros; eapply Con_Mrg_L; solver4.
+Qed.
+
+End papp_consistent.
+
+(** * Weakening Lemma *)
+
+Lemma typing_weakening_gen :
+  forall G E F e A dir,
+    typing (E ++ G) e dir A ->
+    uniq (E ++ F ++ G) ->
+    typing (E ++ F ++ G) e dir A.
+Proof.
+  introv Typ. gen F.
+  dependent induction Typ; introv Env; eauto.
+  pick fresh x and apply Ty_Lam.
+  rewrite_env (([(x,A)] ++ E) ++ F ++ G).
+  apply H0; eauto.
+  solve_uniq.
+Qed.
+
+Lemma typing_weakening :
+  forall E F e A dir,
+    typing E e dir A ->
+    uniq (F ++ E) ->
+    typing (F ++ E) e dir A.
+Proof.
+  intros.
+  rewrite_env (nil ++ F ++ E).
+  eapply typing_weakening_gen; eauto.
+Qed.
+
+(** * Subsitution Lemma *)
+
+Lemma typing_uniq :
+  forall E e T,
+    typing E e Inf T -> uniq E.
+Proof.
+  introv Typ.
+  induction Typ; eauto.
+  - pick fresh x.
+    assert (J: uniq ((one (x,A)) ++ T)); eauto.
+    dependent destruction J; eauto.
+Qed.
+
+Lemma fv_open_lower :
+  forall e1 e2 k,
+    fv e1 [<=] fv (open_rec k e2 e1).
+Proof with auto.
+  intros.
+  generalize dependent k.
+  induction e1; intros; simpl; try fsetdec...
+  - specialize (IHe1_1 k).
+    specialize (IHe1_2 k).
+    fsetdec...
+  - specialize (IHe1_1 k).
+    specialize (IHe1_2 k).
+    fsetdec...
+Qed.
+
+Lemma fv_in_dom :
+  forall T e A dir,
+    typing T e dir A -> fv e [<=] dom T.
+Proof.
+  introv Typ.
+  dependent induction Typ; simpl; try fsetdec; eauto.
+  - apply binds_In in H0.
+    fsetdec.
+  - pick fresh x. 
+    assert ((fv (open e x)) [<=] (dom ((one (x, A)) ++ T))) by eauto.
+    simpl in *.
+    assert (fv e [<=] fv (open e x)).
+    eapply fv_open_lower.
+    assert (fv e [<=] add x (dom T)).
+    fsetdec.
+    eapply add_notin_context; eauto.
+Qed.    
+
+Lemma subst_value :
+  forall e z u A ,
+    typing nil e Inf A -> substitution z u e = e.
+Proof with auto.
+  intros.
+  apply fv_in_dom in H...
+  simpl in H...
+  eapply subst_fresh; eauto.
+  fsetdec.
+Qed.
+
+(** substitution lemma, 
+stating that substituting a (closed, well-typed) term s for a variable x in a term t preserves the type of t *)
+
+Lemma substitution_lemma :
+   forall F E x v e A B C dir,
+    typing (F ++ [(x, A)] ++ E) e dir B ->
+    typing nil v Inf C ->
+    isosub C A ->
+    (exists D, typing (F ++ E) (substitution x v e) dir D /\ isosub D B).
+Proof.
+  introv Typ Typv Isub. remember (F ++ [(x, A)] ++ E) as E'. gen F.
+  induction Typ; intros; simpl; subst; eauto.
+  - Case "Var".
+    destruct (x0 == x); eauto. subst.
+    eapply binds_mid_eq in H0; eauto. subst.
+    exists C. split; eauto.
+    eapply typing_weakening; eauto.
+    rewrite_env (E ++ nil).
+    eapply typing_weakening; eauto.
+    solve_uniq.
+  - Case "Lam".
+    exists (Arr A0 B). split; eauto.
+    eapply (Ty_Lam (union L (singleton x))); eauto. intros.
+    pose proof (H0 x0) as IH.
+    exploit IH; eauto. intros IH'. destruct_conjs.
+    rewrite_env (([(x0, A0)] ++ F) ++ E).
+    rewrite subst_open_var; eauto 3.
+    eapply isosub_to_sub1 in H3.
+    eapply typing_chk_sub; eauto.
+  - Case "Rcd".
+    pose proof (IHTyp F) as IH. exploit IH; eauto. intros IH'.
+    destruct IH'. destruct H. exists (Rcd l x0). split; eauto.
+  - Case "Ann".
+    exists A0. split; eauto.
+    pose proof (IHTyp F) as IH. destruct IH; eauto. destruct_conjs.
+    eapply Ty_Ann; eauto. eapply isosub_to_sub1 in H0.
+    eapply typing_chk_sub; eauto.
+  - Case "App".
+    pose proof (IHTyp1 F) as IH1. pose proof (IHTyp2 F) as IH2.
+    destruct IH1; destruct IH2; eauto. destruct_conjs.
+    eapply uunisub_sound_appsub in H.
+    eapply appsub_iso_v in H; eauto. destruct H. destruct H.
+    exists x2. split; eauto. eapply Ty_App; eauto.
+    eapply uunisub_complete_appsub; eauto.
+  - Case "Prj".
+    pose proof (IHTyp F) as IH. exploit IH; eauto. intros IH'.
+    destruct IH'. destruct H0.
+    eapply uunisub_sound_appsub in H.
+    eapply appsub_iso_l in H; eauto. destruct H. destruct H.
+    exists x1. split; eauto. eapply Ty_Prj; eauto.
+    eapply uunisub_complete_appsub; eauto.
+  - Case "Merge".
+    pose proof (IHTyp1 F) as IH1. pose proof (IHTyp2 F) as IH2.
+    destruct IH1; destruct IH2; eauto. destruct_conjs.
+    exists (And x0 x1). split; eauto.
+    eapply Ty_Mrg; eauto. eapply disjoint_iso_l; eauto.
+  - Case "Merge V".
+    exists (And A0 B). split; eauto.
+    pose proof (subst_value u1 x v _ Typ1) as Rw1.
+    pose proof (subst_value u2 x v _ Typ2) as Rw2.
+    rewrite Rw1. rewrite Rw2.
+    eapply Ty_Mrg_Uv; eauto.
+  - Case "Sub".
+    pose proof (IHTyp F). destruct H0; eauto. destruct H0.
+    exists B. split; eauto. eapply isosub_to_sub1 in H1.
+    eapply Ty_Sub; eauto. eapply sub_transitivity; eauto.
+Qed.
+
+(** * Preservation *)
+Section papp_preservation.
+
+Lemma papp_uvalue_v :
+  forall v vl e A B,
+    value v -> value vl ->
+    typing nil v Inf A -> typing nil vl Inf B ->
+    papp v (Av vl) e ->
+    uvalue e.
+Proof.
+  introv Val Vall Typ Typl Pa. gen A B.
+  dependent induction Pa; intros; eauto 3.
+  - dependent destruction Val. dependent destruction Typ; eauto.
+  - dependent destruction Val. dependent destruction Typ; eauto 3.
+  - dependent destruction Val. dependent destruction Typ; eauto 3.
+  - eapply Uv_Mrg;
+    dependent destruction Val; dependent destruction Typ; eauto 3.
+Qed.
+
+Lemma papp_uvalue_l :
+  forall v l e A,
+    value v ->
+    typing nil v Inf A ->
+    papp v (Al l) e ->
+    uvalue e.
+Proof.
+  introv Val Typ Pa. gen A.
+  dependent induction Pa; intros; eauto 3.
+  - dependent destruction Val. dependent destruction Typ; eauto.
+  - dependent destruction Val. dependent destruction Typ; eauto 3.
+  - dependent destruction Val. dependent destruction Typ; eauto 3.
+  - eapply Uv_Mrg;
+    dependent destruction Val; dependent destruction Typ; eauto 3.
+Qed.
+
+
+Ltac solver1 := repeat match goal with
+                       | [Typ: typing nil ?v Inf ?A, Val: value ?v, Pt: ptype ?v _ |- _] =>
+                           (pose proof (typing_to_ptype _ _ (value_is_uvalue _ Val) Typ); subst_ptype; clear Pt)
+                       | Typ: typing nil ?v Inf ?A, Val: value ?v, At: atype (Av ?v) _ |- _ =>
+                           pose proof (typing_to_atype _ _ Val Typ);
+                           subst_atype; clear At
+                       end.
+
+Lemma papp_preservation_v :
+  forall v vl e A B C,
+    value v -> value vl ->
+    typing nil v Inf A ->
+    typing nil vl Inf B ->
+    appsub (Some (Avt B)) A C ->
+    papp v (Av vl) e ->
+    (exists D, typing nil e Inf D /\ isosub D C).
+Proof.
+  introv Val Vall Typ Typl As Pa. gen A B C.
+  dependent induction Pa; intros.
+  - Case "Lit Toplike".
+    dependent destruction Typ. exists B. split.
+    + eapply Ty_Ann; eauto. eapply typing_chk_sub; eauto.
+      eapply sub_toplike_super; eauto.
+    + dependent destruction As; eauto. dependent destruction H. auto.
+  - Case "Lam".
+    repeat dependent destruction Typ. dependent destruction As.
+    dependent destruction Val.
+    match goal with
+    | [H: sub (Arr _ _) (Arr _ _) |- _] => (dependent destruction H; eauto)
+    end.
+    exists D. split; eauto.
+    match goal with
+    | [H: casting _ _ _ |- _] => (eapply casting_preservation in H; eauto; destruct H; destruct H)
+    end.
+    pick fresh y. rewrite (subst_intro y); eauto.
+    assert (Fr': y `notin` L) by eauto.
+    pose proof (H4 y Fr').
+    rewrite_env (nil ++ [(y, A)] ++ nil) in H8.
+    pose proof (substitution_lemma nil nil y v' (open e y) A B x Chk) as Sl.
+    destruct Sl as [x' Sl']; eauto. destruct Sl'.
+    eapply Ty_Ann; eauto.
+    eapply isosub_to_sub1 in H10; eauto.
+    eapply typing_chk_sub; eauto.
+    eapply sub_transitivity; eauto 3.
+  - Case "Merge L".
+    dependent destruction Val. dependent destruction Typ;
+      dependent destruction As; eauto 3; solver1; eauto.      
+  - Case "Merge R".
+    dependent destruction Val. dependent destruction Typ;
+      dependent destruction As; eauto 3; solver1; eauto.
+  - Case "Merge P".
+    dependent destruction Val. dependent destruction Typ.
+    + solver1.
+      dependent destruction As; eauto.
+      exploit (IHPa1 Val1 _ Vall); eauto.
+      exploit (IHPa2 Val2 _ Vall); eauto.
+      intros IH2 IH1.
+      destruct_conjs. exists (And IH1 IH2). split; eauto.
+      eapply Ty_Mrg; eauto.
+      assert (disjoint C1 C2). eapply disjoint_appsub; eauto.
+      eapply disjoint_iso_l; eauto.
+    + solver1.
+      dependent destruction As; eauto.
+      exploit (IHPa1 Val1 _ Vall); eauto.
+      exploit (IHPa2 Val2 _ Vall); eauto.
+      intros IH2 IH1.
+      destruct_conjs. exists (And IH1 IH2). split; eauto.
+      pose proof (papp_uvalue_v _ _ _ _ _ Val1 Vall Typ1 Typl Pa1).
+      pose proof (papp_uvalue_v _ _ _ _ _ Val2 Vall Typ2 Typl Pa2).
+      eapply Ty_Mrg_Uv; eauto 3.
+      pose proof (papp_consistent_v v1 v2 vl0 e1 e2 A0 B0 B1) as Pc.
+      eapply Pc; eauto.    
+Qed.
+
+
+Ltac solver2 := repeat match goal with
+                       | [Typ: typing nil ?v Inf ?A, Val: value ?v, Pt: ptype ?v _ |- _] =>
+                           (pose proof (typing_to_ptype _ _ (value_is_uvalue _ Val) Typ); subst_ptype; clear Pt)
+                       | At: atype (Al _) _ |- _ =>
+                           dependent destruction At
+                  end.
+
+Lemma selector_as :
+  forall A B1 B2 S,
+    appsub (Some S) A B1 ->
+    selectorT A B2 ->
+    B1 = B2.
+Proof.
+  introv As SeT.
+  dependent destruction SeT; eauto.
+  - dependent destruction As; eauto.
+  - dependent destruction As; eauto.
+Qed.
+
+Lemma papp_preservation_l :
+  forall v l e A B,
+    value v ->
+    typing nil v Inf A ->
+    appsub (Some (Alt l)) A B ->
+    papp v (Al l) e ->
+    (exists C, typing nil e Inf C /\ isosub C B).
+Proof.
+  introv Val Typ As Pa. gen A B.
+  dependent induction Pa; intros.
+  - Case "Toplike".
+    dependent destruction Val.
+    dependent destruction H.
+    * destruct H1.
+      ** eexists. dependent destruction Typ. dependent destruction As; eauto.
+      ** eexists. dependent destruction Typ. dependent destruction As; eauto.
+    * destruct H1.
+      ** dependent destruction Typ. dependent destruction As; eauto.
+         exists A. split; eauto.
+         eapply Ty_Ann; eauto. eapply typing_chk_sub; eauto.
+         eapply sub_toplike_super; eauto.
+      ** dependent destruction Typ. dependent destruction As; eauto.
+         exists A. split; eauto.
+         eapply Ty_Ann; eauto. eapply typing_chk_sub; eauto.
+         eapply sub_toplike_super; eauto.
+  - Case "Prj".
+    dependent destruction Typ. dependent destruction As.
+    exists A. split; eauto.
+  - Case "Merge L".
+    dependent destruction Val. dependent destruction Typ;
+      dependent destruction As; eauto 3; solver2; eauto.
+  - Case "Merge R".
+    dependent destruction Val. dependent destruction Typ;
+      dependent destruction As; eauto 3; solver2; eauto.
+  - Case "Merge P".
+    dependent destruction Val. dependent destruction Typ.
+    + solver2.
+      dependent destruction As; eauto.
+      exploit (IHPa1 l Val1); eauto.
+      exploit (IHPa2 l Val2); eauto.
+      intros IH2 IH1.
+      destruct_conjs. exists (And IH1 IH2). split; eauto.
+      eapply Ty_Mrg; eauto.
+      assert (disjoint C1 C2). eapply disjoint_appsub; eauto.
+      eapply disjoint_iso_l; eauto.
+    + solver2.
+      dependent destruction As; eauto.
+      exploit (IHPa1 l Val1); eauto.
+      exploit (IHPa2 l Val2); eauto.
+      intros IH2 IH1.
+      destruct_conjs. exists (And IH1 IH2). split; eauto.
+      pose proof (papp_uvalue_l v1 l e1).
+      pose proof (papp_uvalue_l v2 l e2).
+      eapply Ty_Mrg_Uv; eauto 3.
+      pose proof (papp_consistent_l _ _ _ _ _ _ _ Val1 Val2 Typ1 Typ2 Pa1 Pa2) as Pc.
+      eapply Pc; eauto.
+      Unshelve. auto. auto.
+Qed.
+
+End papp_preservation.
+
+(** * Progress *)
+
+Lemma papp_progress_v :
+  forall f v A B C,
+    value f -> value v ->
+    typing nil f Inf A -> typing nil v Inf B ->
+    appsub (Some (Avt B)) A C ->
+    exists e, papp f (Av v) e.
+Proof.
+  introv Vf Vv Tf Tv As. gen A B C v.
+  induction Vf; intros.
+  - Case "Anno".
+    destruct H.
+    + SCase "Lit".
+      repeat dependent destruction Tf.
+      dependent destruction H1; eauto. dependent destruction As; eauto.
+    + SCase "Lam".
+      repeat dependent destruction Tf.
+      dependent destruction H2; eauto.
+      * dependent destruction As; eauto.
+      * destruct (toplike_decidable D); eauto.
+        dependent destruction As; eauto.
+        assert (Sub: sub B1 A1) by (eapply sub_transitivity; eauto).
+        pose proof (casting_progress' _ _ _ Vv Tv Sub) as Ct. destruct Ct.
+        eexists. eapply Pa_Lam; eauto.
+  - Case "Rcd".
+    dependent destruction Tf; eauto.
+  - Case "Merge".
+    dependent destruction As.
+    + inversion Tf.
+    + dependent destruction Tf.
+      * pose proof (IHVf1 _ Tf1 _ _ As _ Vv Tv) as IH. destruct IH.
+        eexists. eapply Pa_Mrg_L; eauto.
+      * pose proof (IHVf1 _ Tf1 _ _ As _ Vv Tv) as IH. destruct IH.
+        eexists. eapply Pa_Mrg_L; eauto.
+    + dependent destruction Tf.
+      * pose proof (IHVf2 _ Tf2 _ _ As _ Vv Tv) as IH. destruct IH.
+        eexists. eapply Pa_Mrg_R; eauto.
+      * pose proof (IHVf2 _ Tf2 _ _ As _ Vv Tv) as IH. destruct IH.
+        eexists. eapply Pa_Mrg_R; eauto.
+    + dependent destruction Tf.
+      * pose proof (IHVf1 _ Tf1 _ _ As1 _ Vv Tv) as IH1. destruct IH1.
+        pose proof (IHVf2 _ Tf2 _ _ As2 _ Vv Tv) as IH2. destruct IH2.
+        eexists. eapply Pa_Mrg_P; eauto.
+      * pose proof (IHVf1 _ Tf1 _ _ As1 _ Vv Tv) as IH1. destruct IH1.
+        pose proof (IHVf2 _ Tf2 _ _ As2 _ Vv Tv) as IH2. destruct IH2.
+        eexists. eapply Pa_Mrg_P; eauto.
+Qed.
+
+Lemma papp_progress_l :
+  forall v A B l,
+    value v ->
+    typing nil v Inf A ->
+    appsub (Some (Alt l)) A B ->
+    exists e, papp v (Al l) e.
+Proof.
+  introv Val Typ As. gen A B l.
+  induction Val; intros.
+  - Case "Ann". destruct H.
+    + SCase "Lit".
+      repeat dependent destruction Typ.
+      dependent destruction H1; eauto. dependent destruction As; eauto.
+    + SCase "Lam".
+      repeat dependent destruction Typ.
+      dependent destruction H2; eauto. dependent destruction As; eauto.
+  - Case "Rcd".
+    dependent destruction Typ; eauto.
+    dependent destruction As. eauto.
+  - Case "Merge".
+    dependent destruction As.
+    + inversion Typ.
+    + dependent destruction Typ.
+      * pose proof (IHVal1 _ Typ1 _ _ As) as IH. destruct IH.
+        eexists. eapply Pa_Mrg_L; eauto.
+      * pose proof (IHVal1 _ Typ1 _ _ As) as IH. destruct IH.
+        eexists. eapply Pa_Mrg_L; eauto.
+    + dependent destruction Typ.
+      * pose proof (IHVal2 _ Typ2 _ _ As) as IH. destruct IH.
+        eexists. eapply Pa_Mrg_R; eauto.
+      * pose proof (IHVal2 _ Typ2 _ _ As) as IH. destruct IH.
+        eexists. eapply Pa_Mrg_R; eauto.
+    + dependent destruction Typ.
+      * pose proof (IHVal1 _ Typ1 _ _ As1) as IH1. destruct IH1.
+        pose proof (IHVal2 _ Typ2 _ _ As2) as IH2. destruct IH2.
+        eexists. eapply Pa_Mrg_P; eauto.
+      * pose proof (IHVal1 _ Typ1 _ _ As1) as IH1. destruct IH1.
+        pose proof (IHVal2 _ Typ2 _ _ As2) as IH2. destruct IH2.
+        eexists. eapply Pa_Mrg_P; eauto.
+Qed.
