README.txt
@@ -1,0 +1,13 @@
+core: a type sound calculus with applicative subtyping
+
+core+record: add record types
+
+core+record+disjoint: a type sound and coherent calculus with disjointness
+
+*/typeset: typeset files, run "rake" to generate pdf
+
+*/Proof: coq formalization, run "make" to generate coqdoc htmls
+
+implementation: interpreter and compiler in Racket
+
+subtyping: Haskell's implementation of applicative subtyping
